Move files to experiment

state/experiments/FlagBasedEffPoly.fst
@@ -1,39 +1,155 @@
 module FlagBasedEffPoly
 
-open FStar.Monotonic.Heap
-open FStar.ST
+open Labeled.Monotonic.Heap
+open Labeled.MST
+open Witnessable
+open TargetLang
+open STLC 
 
-type myref a =
-  Heap.mref a (fun _ _ -> True)
+(** for the very general idea, look into experiments/FlagBasedEffPoly.fst **)
 
 type fo_ctx =
-  // fl:erased tflag -> (** we don't have flag yets for ST **)
-  #inv:(heap -> Type0) -> (** invariant on the heap **)
-  #prref:((#a:Type0) -> ref a -> Type0) -> (** predicate that refines references **)
-  read : ((#a:Type0) -> x:ref a -> ST a (fun h0 -> inv h0 /\ prref x) (fun _ _ h1 -> inv h1)) ->
-  write : ((#a:Type0) -> x:ref a -> v:a -> ST unit (fun h0 -> inv h0 /\ prref x) (fun _ _ h1 -> inv h1)) ->
-  alloc : ((#a:Type0) -> init:a -> ST (ref a) (fun h0 -> inv h0) (fun _ r h1 -> inv h1 /\ prref r)) ->
-  ST unit (inv) (fun _ _ -> inv)
+  #inv:(lheap -> Type0) -> (** invariant on the heap **)
+  #prref: (#a:Type -> #rel:_ -> mref a rel -> Type0) ->
+  #hrel:FStar.Preorder.preorder lheap ->
+ // #hrel:(rel:(lheap -> lheap -> Type0){FStar.Preorder.transitive rel}) -> (** because of the hrel, we may not need the flag because even if the context uses operations directly, it cannot prove that it preserves the hrel**)
+  (** ^ if this predicate would be also over heaps, then the contexts needs witness&recall in HO settings **)
+  read :  ((#t:typ0) -> r:ref (elab_typ0 t) -> 
+            ST (elab_typ0 t) 
+              (requires (fun h0 -> inv h0 /\ prref r))
+              (ensures  (fun h0 v h1 -> h0 `hrel` h1 /\ inv h1 /\ (** prref r /\**) (elab_typ0_tc t).satisfy_refinement v prref))) -> // sel h1 r == v /\
+  write : ((#t:typ0) -> r:ref (elab_typ0 t) -> v:(elab_typ0 t) -> 
+            ST unit
+              (requires (fun h0 -> inv h0 /\ prref r /\ (elab_typ0_tc t).satisfy_refinement v prref))
+              (ensures  (fun h0 _ h1 -> h0 `hrel` h1 /\ inv h1 (**/\ prref r /\ (elab_typ0_tc t).satisfy_refinement v prref **)))) -> // /\ sel h1 r == v 
+  alloc : ((#t:typ0) -> init:(elab_typ0 t) -> 
+            ST (ref (elab_typ0 t)) 
+              (requires (fun h0 -> inv h0 /\ (elab_typ0_tc t).satisfy_refinement init prref))
+              (ensures  (fun h0 r h1 -> h0 `hrel` h1 /\ inv h1 /\ prref r (** /\ (elab_typ0_tc t).satisfy_refinement init prref **)))) -> // sel h1 r == init /\  
+  (** type of the context: *)
+  unit -> ST unit (inv) (fun h0 _ h1 -> inv h1 /\ h0 `hrel` h1)
 
-val ctx1 : fo_ctx
-let ctx1 my_read my_write my_alloc =
+(** Checking if there exists read, write, alloc so that we can instantiate the polymorphic context **)
+
+unfold
+let is_low_pred' r : pred:heap_predicate{stable pred} = (* F* being silly. There is an SMTPat on is_low_pred_stable **)
+  let pred = is_low_pred r in
+  is_low_pred_stable r;
+  pred
+ 
+let check_instantiating_the_context (ctx:fo_ctx) = 
+  ctx
+    #(fun h -> inv_low_contains h)
+    #(fun r -> witnessed (contains_pred r) /\ witnessed (is_low_pred' r)) 
+    #(fun h0 h1 -> modifies_only_label Low h0 h1 /\ modifies_classification Set.empty h0 h1)
+    (fun #t r -> (* READ *)
+      let h0 = get () in
+      mst_recall (contains_pred r); 
+      mst_recall (is_low_pred r);
+      let v = read r in
+      assert ((elab_typ0_tc t).satisfy v h0 contains_pred);
+      assert ((elab_typ0_tc t).satisfy v h0 is_low_pred);
+      assume ((elab_typ0_tc t).satisfy_refinement v (fun r' -> witnessed (contains_pred r') /\ witnessed (is_low_pred' r'))); (** one can create witnesses using the previous assertions **)
+      v) 
+    (fun #t r v -> (* WRITE *)
+      mst_recall (contains_pred r); 
+      mst_recall (is_low_pred r); 
+      let h0 = get () in
+      assert ((elab_typ0_tc t).satisfy_refinement v (fun r' -> witnessed (contains_pred r') /\ witnessed (is_low_pred' r')));
+      assume (shallowly_contained_low v #(elab_typ0_tc t) h0); (** one has to recall on v. a method on witnessable, that given a `witnessed pred`, returns a `satisfy pred`. **)
+      elab_write r v)
+    (fun #t init -> (* ALLOC *)
+      let h0 = get () in
+      assert ((elab_typ0_tc t).satisfy_refinement init (fun r' -> witnessed (contains_pred r') /\ witnessed (is_low_pred' r')));
+      assume (shallowly_contained_low init #(elab_typ0_tc t) h0); (** one has to recall on init **)
+      let r = elab_alloc init in 
+      mst_witness (contains_pred r); mst_witness (is_low_pred r);
+      r)
+
+
+(** TODO: Can the context easily/automatically work with the pre- and post-conditions? **)
+
+
+open FStar.Tactics
+
+(** CA: this test fails if the relation is not reflexive **)
+val ctx_pure : fo_ctx
+let ctx_pure #inv #_ #hrel my_read my_write my_alloc () : ST unit (inv) (fun h0 _ h1 -> inv h1 /\ h0 `hrel` h1) by (
+  explode ();
+     let bi = nth_binder (-2) in
+     let (_, fl) = destruct_and bi in
+     clear bi;
+     let fl' = instantiate fl (nth_binder (-3)) in
+     clear fl;
+     let fl'' = instantiate fl' (nth_binder (-4)) in
+     clear fl';
+  dump "H"
+)=
+  ()
+  
+  
+val ctx_update_ref_test : fo_ctx
+let ctx_update_ref_test my_read my_write my_alloc () =
   let x = my_alloc 5 in
   let y = my_read x in
-  my_write x (y+1);
+  my_write #TNat x (y+1);
   ()
 
-type rho_ctx =
-  // fl:erased tflag ->
-  #inv:(heap -> Type0) ->
-  #prref:((#a:Type0) -> myref a -> Type0) ->
-  read : ((#a:Type0) -> x:ref a -> ST a (fun h0 -> inv h0 /\ prref x) (fun _ _ h1 -> inv h1)) ->
-  write : ((#a:Type0) -> x:ref a -> v:a -> ST unit (fun h0 -> inv h0 /\ prref x) (fun _ _ h1 -> inv h1)) ->
-  alloc : ((#a:Type0) -> init:a -> ST (ref a) (fun h0 -> inv h0) (fun _ r h1 -> inv h1 /\ prref r)) ->
-  ST (unit -> ST unit (inv) (fun _ _ -> inv)) (inv) (fun _ _ -> inv)
+type ho_ctx1 = (** only the type of the context is different **)
+  #inv:(lheap -> Type0) -> (** invariant on the heap **)
+  #prref: (#a:Type -> #rel:_ -> mref a rel -> Type0) ->
+  #hrel:(FStar.Preorder.preorder lheap) ->
+  (** ^ if this predicate would be also over heaps, then the contexts needs witness&recall in HO settings **)
+  read :  ((#t:typ0) -> r:ref (elab_typ0 t) -> 
+            ST (elab_typ0 t) 
+              (requires (fun h0 -> inv h0 /\ prref r))
+              (ensures  (fun h0 v h1 -> h0 `hrel` h1 /\ inv h1 /\ (** prref r /\**) (elab_typ0_tc t).satisfy_refinement v prref))) -> // sel h1 r == v /\
+  write : ((#t:typ0) -> r:ref (elab_typ0 t) -> v:(elab_typ0 t) -> 
+            ST unit
+              (requires (fun h0 -> inv h0 /\ prref r /\ (elab_typ0_tc t).satisfy_refinement v prref))
+              (ensures  (fun h0 _ h1 -> h0 `hrel` h1 /\ inv h1 (**/\ prref r /\ (elab_typ0_tc t).satisfy_refinement v prref **)))) -> // /\ sel h1 r == v 
+  alloc : ((#t:typ0) -> init:(elab_typ0 t) -> 
+            ST (ref (elab_typ0 t)) 
+              (requires (fun h0 -> inv h0 /\ (elab_typ0_tc t).satisfy_refinement init prref))
+              (ensures  (fun h0 r h1 -> h0 `hrel` h1 /\ inv h1 /\ prref r (** /\ (elab_typ0_tc t).satisfy_refinement init prref **)))) -> // sel h1 r == init /\  
+  (** type of the context: *)
+  rr:ref (ref int) -> ST (r:ref int -> ST unit (fun h0 -> inv h0 /\ prref r) (fun h0 _ h1 -> inv h1 /\ hrel h0 h1))
+    (requires (fun h0 -> inv h0 /\ prref rr))
+    (ensures  (fun h0 _ h1 -> inv h1 /\ hrel h0 h1))
 
-val ctx2 : rho_ctx
-let ctx2 #_ #prref my_read my_write my_alloc =
-  let x : ref int = my_alloc 5 in
-  (fun () -> 
-    assert (prref x); (** why is this working? because ref cannot change. the predicate is not over the heap **)
-    let y = my_read x in ())
+val ctx_update_multiple_refs_test : ho_ctx1
+let ctx_update_multiple_refs_test #inv #prref #hrel my_read my_write my_alloc x y =
+  let ix = my_read #(TRef TNat) x in
+  my_write #(TRef TNat) x y;
+  my_write #TNat y ((my_read #TNat y) + 5);
+  ()
+
+
+type ho_ctx2 =
+  #inv:(lheap -> Type0) -> (** invariant on the heap **)
+  #prref: (#a:Type -> #rel:_ -> mref a rel -> Type0) ->
+  #hrel:(rel:(lheap -> lheap -> Type0){FStar.Preorder.transitive rel}) -> (** because of the hrel, we may not need the flag because even if the context uses operations directly, it cannot prove that it preserves the hrel**)
+  (** ^ if this predicate would be also over heaps, then the contexts needs witness&recall in HO settings **)
+  read :  ((#t:typ0) -> r:ref (elab_typ0 t) -> 
+            ST (elab_typ0 t) 
+              (requires (fun h0 -> inv h0 /\ prref r))
+              (ensures  (fun h0 v h1 -> inv h1 /\ prref r /\ (elab_typ0_tc t).satisfy_refinement v prref /\ h0 `hrel` h1))) -> // sel h1 r == v /\
+  write : ((#t:typ0) -> r:ref (elab_typ0 t) -> v:(elab_typ0 t) -> 
+            ST unit
+              (requires (fun h0 -> inv h0 /\ prref r /\ (elab_typ0_tc t).satisfy_refinement v prref))
+              (ensures  (fun h0 _ h1 -> inv h1 /\ prref r /\ h0 `hrel` h1 /\ (elab_typ0_tc t).satisfy_refinement v prref))) -> // /\ sel h1 r == v 
+  alloc : ((#t:typ0) -> init:(elab_typ0 t) -> 
+            ST (ref (elab_typ0 t)) 
+              (requires (fun h0 -> inv h0 /\ (elab_typ0_tc t).satisfy_refinement init prref))
+              (ensures  (fun h0 r h1 -> inv h1 /\ prref r /\ h0 `hrel` h1 /\ (elab_typ0_tc t).satisfy_refinement init prref))) -> // sel h1 r == init /\  
+  (** type of the context: *)
+  rr:ref ((ref int) * (ref int)) -> ST (unit -> ST unit (fun h0 -> inv h0) (fun h0 _ h1 -> inv h1 /\ h0 `hrel` h1))
+    (requires (fun h0 -> inv h0 /\ prref rr))
+    (ensures  (fun h0 _ h1 -> inv h1 /\ h0 `hrel` h1))
+
+val ctx_HO_test1 : ho_ctx2
+let ctx_HO_test1 #inv #prref my_read my_write my_alloc rr =
+  let (x', x'') = my_read #(TPair (TRef TNat) (TRef TNat)) rr in
+  my_write #(TPair (TRef TNat) (TRef TNat)) rr (x', x');
+  (fun _ ->
+    my_write #(TPair (TRef TNat) (TRef TNat)) rr (x', x''))
